More progress on DuplexPCM, only frame_compatible missing

pulse/ulib/experimental/Steel.FramingDuplex.PCM.fst
@@ -31,7 +31,11 @@ type t (p:dprot) =
  | Nil
 
 let ahead (#p:dprot) (q q':dprot) (s:trace p q) (s':trace p q') : prop
-  = squash ({ to = q'; tr = s'} `extended_to` { to = q; tr = s })
+  = ({ to = q'; tr = s'} `extended_to` { to = q; tr = s }) /\ True
+
+let ahead_refl (#p:dprot) (q:dprot) (s:trace p q)
+  : Lemma (ahead q q s s)
+  = ()
 
 let rec trace_length #p #q (s:trace p q) : Tot nat (decreases s) = match s with
   | Waiting _ -> 0
@@ -104,9 +108,9 @@ let endpoint_b (#p:dprot) (c:chan p) (next:dprot) (tr:trace p next) =
 // From Basics
 
 assume
-val cond (#a:Type) (b:bool) (p: bool -> slprop) (q: bool -> a -> slprop)
-         (then_: (unit -> SteelT a (p true) (q true)))
-         (else_: (unit -> SteelT a (p false) (q false)))
+val cond (#a:Type) (b:bool) (p: (b':bool{b == b'}) -> slprop) (q: bool -> a -> slprop)
+         (then_: (squash (b == true) -> SteelT a (p true) (q true)))
+         (else_: (squash (b == false) -> SteelT a (p false) (q false)))
   : SteelT a (p b) (q b)
 
 assume
@@ -141,18 +145,213 @@ val select_refine (#p:dprot)
              (pts_to r x)
              (fun v -> pts_to r (f v))
 
-let next_message (#p:dprot) (#q:dprot{more q}) (tr:trace p q)
-  (tr':partial_trace_of p{trace_length tr'.tr > trace_length tr})
-  : (x:msg_t q)
-  = admit()
+let rec is_trace_prefix
+  (#from:protocol unit) (#to #to':protocol unit)
+  (tr:trace from to)
+  (tr':trace from to')
+  : Tot prop
+    (decreases tr)
+  = match tr with
+    | Waiting _ -> True
+    | Message _ x _ tail ->
+      match tr' with
+      | Waiting _ -> False
+      | Message _ x' _ tail' -> x == x' /\ is_trace_prefix tail tail'
 
-let extend_node_a_r (#p:dprot) (#q:dprot{more q /\ is_recv q}) (tr:trace p q)
-  (tr':partial_trace_of p{trace_length tr'.tr > trace_length tr})
+let rec lemma_is_trace_prefix_refl
+  (#from #to:protocol unit)
+  (tr:trace from to)
+  : Lemma (ensures is_trace_prefix tr tr)
+          (decreases tr)
+  = match tr with
+    | Waiting _ -> ()
+    | Message _ _ _ tail -> lemma_is_trace_prefix_refl tail
+
+let rec lemma_is_trace_prefix_extend (#from #to #to':protocol unit)
+  (tr:trace from to)
+  (tr':trace from to')
+  (x:msg_t to')
+  : Lemma (requires is_trace_prefix tr tr' /\ more_msgs to')
+          (ensures is_trace_prefix tr (extend tr' x))
+          (decreases tr)
+  = match tr with
+    | Waiting _ -> ()
+    | Message _ msg _ tail ->
+      match tr' with
+      | Message from' msg' to' tail' -> lemma_is_trace_prefix_extend tail tail' x
+
+let lemma_ahead_msg_msg_inversion
+  (#from:dprot) (#to #to':dprot)
+  (tr:trace from to)
+  (tr':trace from to')
+  : Lemma (requires Message? tr /\ Message? tr' /\ is_trace_prefix tr tr')
+          (ensures Message?.x tr == Message?.x tr' /\ is_trace_prefix (Message?._3 tr) (Message?._3 tr'))
+  = let Message _ x _ tail = tr in
+    let Message _ x' _ tail' = tr' in
+    let l = ({to = to; tr = tr}) in
+    let r = ({to = to'; tr = tr'}) in
+    let open FStar.ReflexiveTransitiveClosure in
+    let stable1 (z:partial_trace_of from) : Type0 = Message? z.tr /\ Message?.x z.tr == x in
+    let aux1 (y z:partial_trace_of from)
+      : Lemma (requires stable1 y /\ next y z)
+              (ensures stable1 z)
+      = ()
+    in Classical.forall_intro_2 (Classical.move_requires_2 aux1);
+    stable_on_closure next stable1 ();
+    assert (x == x');
+    let stable2 (z:partial_trace_of (step from x)) : Type0 =
+      is_trace_prefix tail z.tr
+    in
+    let aux2 (y z:partial_trace_of (step from x))
+      : Lemma (requires stable2 y /\ next y z)
+              (ensures stable2 z)
+      = Classical.forall_intro (Classical.move_requires (lemma_is_trace_prefix_extend tail y.tr))
+    in Classical.forall_intro_2 (Classical.move_requires_2 aux2);
+    stable_on_closure next stable2 ()
+
+let rec next_message_aux
+  (#from:dprot) (#to #to':dprot)
+  (tr:trace from to)
+  (tr':trace from to'{trace_length tr' > trace_length tr /\ is_trace_prefix tr tr'})
+  : Tot (msg_t to)
+        (decreases tr)
+  = match tr with
+    | Waiting _ ->
+        assert (Message? tr');
+        Message?.x tr'
+    | Message _ x to tail ->
+      let Message _ x' to' tail' = tr' in
+      lemma_ahead_msg_msg_inversion tr tr';
+      next_message_aux tail tail'
+
+let lemma_ahead_implies_trace_prefix
+  (#from:dprot) (#to #to':dprot)
+  (tr:trace from to)
+  (tr':trace from to')
+  : Lemma (requires ahead to' to tr' tr)
+          (ensures is_trace_prefix tr tr')
+  = let stable (z:partial_trace_of from) : Type0 = is_trace_prefix tr z.tr in
+    let aux (y z:partial_trace_of from)
+      : Lemma (requires stable y /\ next y z)
+              (ensures stable z)
+      = Classical.forall_intro (Classical.move_requires (lemma_is_trace_prefix_extend tr y.tr))
+   in Classical.forall_intro_2 (Classical.move_requires_2 aux);
+   let open FStar.ReflexiveTransitiveClosure in
+   stable_on_closure next stable ();
+   lemma_is_trace_prefix_refl tr
+
+let next_message
+  (#from:dprot) (#to #to':dprot)
+  (tr:trace from to)
+  (tr':trace from to'{trace_length tr' > trace_length tr /\
+    ahead to' to tr' tr})
+  = lemma_ahead_implies_trace_prefix tr tr';
+    next_message_aux tr tr'
+
+let rec extend_increase_length (#from #to:protocol unit) (t:trace from to{more_msgs to}) (m:next_msg_t to)
+  : Lemma (ensures trace_length (extend t m) == trace_length t + 1)
+          (decreases t)
+  = match t with
+    | Waiting _ -> ()
+    | Message _ _ _ tail -> extend_increase_length tail m
+
+let next_increase_length (#p:dprot) (x y:partial_trace_of p)
+  : Lemma (requires next x y)
+          (ensures trace_length y.tr == trace_length x.tr + 1)
+  = let aux (msg:next_msg_t x.to)
+        : Lemma (requires y.to == step x.to msg /\ y.tr == extend x.tr msg)
+                (ensures trace_length y.tr == trace_length x.tr + 1)
+        = extend_increase_length x.tr msg
+    in Classical.forall_intro (Classical.move_requires aux)
+
+let rec lemma_ahead_is_longer (#p:dprot) (q:dprot) (s:trace p q) (q':dprot) (s':trace p q')
+  : Lemma (requires ahead q q' s s')
+          (ensures trace_length s >= trace_length s')
+  = let open FStar.ReflexiveTransitiveClosure in
+    let l = ({to = q'; tr = s'}) in
+    let r = ({to = q; tr = s}) in
+    let stable_p (x:partial_trace_of p) : Type0 = trace_length x.tr >= trace_length s' in
+    let aux (x y:partial_trace_of p)
+      : Lemma (requires stable_p x /\ next x y)
+              (ensures stable_p y)
+      = next_increase_length x y
+    in Classical.forall_intro_2 (fun x -> Classical.move_requires (aux x));
+    stable_on_closure next stable_p ()
+
+let compatible_a_r_v_is_ahead
+  (#p:dprot) (#q:dprot{is_recv q}) (tr:trace p q)
+  (tr':partial_trace_of p)
+  : Lemma (requires compatible (pcm p) (A_R q tr) (V tr'))
+          (ensures ahead tr'.to q tr'.tr tr)
+  =  let aux (frame:t p) : Lemma
+        (requires composable (A_R q tr) frame /\ compose frame (A_R q tr) == V tr')
+        (ensures ahead tr'.to q tr'.tr tr)
+        = assert (B_R? frame \/ B_W? frame);
+          if B_W? frame then ()
+          else
+            let q' = B_R?.q frame in
+            let tr' = B_R?._1 frame in
+            if trace_length tr' >= trace_length tr then
+              Classical.move_requires (lemma_ahead_is_longer q tr q') tr'
+            else ahead_refl q tr
+    in
+    Classical.forall_intro (Classical.move_requires aux)
+
+  let extend_node_a_r (#p:dprot) (#q:dprot{more q /\ is_recv q}) (tr:trace p q)
+  (tr':partial_trace_of p{trace_length tr'.tr > trace_length tr /\
+    compatible (pcm p) (A_R q tr) (V tr')})
   : (y:t p)
-  = let x = next_message tr tr' in
+  = compatible_a_r_v_is_ahead tr tr';
+    let x = next_message tr tr'.tr in
     let q' = step q x in
     let tr' = extend tr x in
     if is_send q' then A_W q' tr' else A_R q' tr'
+
+let lemma_compatible_a_greater_length (#p:dprot) (q:dprot{is_recv q}) (tr:trace p q) (tr':partial_trace_of p)
+  : Lemma (requires compatible (pcm p) (A_R q tr) (V tr'))
+          (ensures trace_length tr'.tr >= trace_length tr)
+  = compatible_a_r_v_is_ahead tr tr';
+    lemma_ahead_is_longer tr'.to tr'.tr q tr
+
+let lemma_next_injectivity
+  (#p:dprot) (tr tr':partial_trace_of p)
+  (z1 z2:partial_trace_of p)
+  : Lemma (requires tr `extended_to` tr' /\
+            (next tr z1 /\ z1 `extended_to` tr') /\
+            (next tr z2 /\ z2 `extended_to` tr'))
+          (ensures z1 == z2)
+  = admit()
+
+let frame_compatible_a_extend (#p:dprot)
+  (q:dprot{is_recv q /\ more q}) (tr:trace p q)
+  (tr':partial_trace_of p)
+  : Lemma (requires compatible (pcm p) (A_R q tr) (V tr') /\ trace_length tr'.tr > trace_length tr)
+          (ensures frame_compatible (A_R q tr) (V tr') (extend_node_a_r tr tr'))
+  = let x = A_R q tr in
+    let p_tr:partial_trace_of p = {to = q; tr = tr} in
+    let v = V tr' in
+    let y = extend_node_a_r tr tr' in
+    let aux (frame:t p)
+      : Lemma (requires composable x frame /\ v == compose x frame)
+              (ensures composable y frame /\ v == compose y frame)
+      = assert (B_R? frame \/ B_W? frame);
+        if B_W? frame then (
+          let q_w = B_W?.q frame in
+          let tr_w = B_W?._1 frame in
+          assert (tr_w == tr'.tr);
+          // TODO: Likely need to strengthen the pcm
+          // Ahead should also say something like "the "additional suffix" only
+          // contains writes, i.e. you cannot read the future
+          assume (A_R? y);
+          let msg = next_message tr tr_w in
+          let q' = step q msg in
+          let tr_new = extend tr msg in
+          assert (y == A_R q' tr_new);
+          let z' = {to = q'; tr = tr_new} in
+          //assert (({to = q'; tr = tr_new}) `extended_to` ({to = q_w; tr = tr_w}));
+          admit()
+        ) else admit()
+    in Classical.forall_intro (Classical.move_requires aux)
 
 let f_a_r (#p:dprot) (q:dprot{is_recv q /\ more q}) (tr:trace p q)
   (v:t p{compatible (pcm p) (A_R q tr) v})
@@ -160,13 +359,13 @@ let f_a_r (#p:dprot) (q:dprot{is_recv q /\ more q}) (tr:trace p q)
   = match v with
     | A_R q tr -> A_R q tr
     | V tr' ->
-        assume (trace_length tr'.tr >= trace_length tr);
+        lemma_compatible_a_greater_length q tr tr';
         if trace_length tr >= trace_length tr'.tr then
           // No new message yet
           A_R q tr
         else
           let y = extend_node_a_r tr tr' in
-          assume (frame_compatible (A_R q tr) v y);
+          frame_compatible_a_extend q tr tr';
           y
 
 val get_a_r (#p:dprot) (c:chan p) (q:dprot{is_recv q /\ more q}) (tr:trace p q)
@@ -198,15 +397,6 @@ val write_a
   (x:msg_t next)
   :SteelT unit (pts_to r (A_W next tr)) (fun _ -> endpoint_a r (step next x) (extend tr x))
 
-
-// assume
-// val get (#p:dprot) (r:ref (t p) (pcm p)) (v0:erased (t p))
-//   : SteelT (v:(t p){compatible (pcm p) v0 v}) (pts_to r v0) (fun v -> pts_to r v)
-
-// assume
-// val upd (r:ref stepper p) (v0:erased stepper) (v1:stepper { frame_preserving p v0 v1})
-//   : SteelT unit (pts_to r v0) (fun _ -> pts_to r v1)
-
 assume
 val alloc (#p:dprot) (x:t p)
   : Steel (chan p) emp (fun r -> pts_to r x) (fun _ -> squash (compatible (pcm p) x x)) (fun _ _ _ -> True)
@@ -232,7 +422,7 @@ let new_chan p =
   split r v
     (if is_send p then A_W p (empty_trace p) else A_R p (empty_trace p))
     (if is_send p then B_R p (empty_trace p) else B_W p (empty_trace p))
-    (admit()) ();
+    (ahead_refl p (empty_trace p)) ();
   r
 
 val send_a
@@ -265,14 +455,13 @@ let rec recv_a #p c next tr =
     // Problem: The second precondition requires (not b) to typecheck
     (fun b ->
       if b then pts_to c (A_R next tr)
-      else (assume (trace_length tr < trace_length tr'.tr); pts_to c (extend_node_a_r tr tr'))
+      else (pts_to c (extend_node_a_r tr tr'))
     )
     (fun _ x -> endpoint_a c (step next x) (extend tr x))
     (fun _ ->
       change_slprop (pts_to c (A_R next tr)) (endpoint_a c next tr) (fun _ -> ());
       recv_a c next tr)
     (fun _ ->
-      assume (trace_length tr < trace_length tr'.tr);
       let x = next_message tr tr' in
       change_slprop
         (pts_to c (extend_node_a_r tr tr'))
